Copy-paste and customize heap_lang in this repo.
Side effects : use a specific Val constructor for values (many simplifications), native machine integers.

theories/ClockIntegers.v
@@ -1,5 +1,5 @@
-From iris.heap_lang Require Import proofmode notation.
-From iris_time Require Import TimeReceipts MachineIntegers.
+From iris_time.heap_lang Require Import proofmode notation.
+From iris_time Require Import TimeReceipts.
 From stdpp Require Import numbers.
 
 Open Scope Z_scope.
@@ -13,28 +13,32 @@ Section clock_int.
 
   Context `{timeReceiptHeapG Σ}.
   Context (nmax : nat).
-  Context `(nmax ≤ max_int).
+  Context `(nmax ≤ max_mach_int).
 
-  Definition is_clock_int (n : nat) : iProp Σ :=
-    TR n.
+  Definition is_clock_int (n : Z) : iProp Σ :=
+    (⌜0 ≤ n⌝ ∗ TR (Z.to_nat n))%I.
 
   (* Clock integers support addition, which consumes its arguments: *)
-  Lemma clock_int_add_spec n1 n2 :
+  Lemma clock_int_add_spec (n1 n2 : mach_int) :
     TR_invariant nmax -∗
-    {{{ is_clock_int n1 ∗ is_clock_int n2 }}}
-    machine_int_add #n1 #n2
-    {{{ RET #(n1+n2) ; is_clock_int (n1+n2) }}}.
+    {{{ is_clock_int (`n1) ∗ is_clock_int (`n2) }}}
+    #n1 + #n2
+    {{{ H, RET #(LitMachInt ((`n1+`n2) ↾ H)) ; is_clock_int (`n1+`n2) }}}.
   Proof.
-    iIntros "#Htrinv" (Φ) "!# (H1 & H2) Post".
-    iAssert (TR (n1+n2)) with "[H1 H2]" as "H" ; first by (rewrite TR_plus ; iFrame).
-    iDestruct (TR_lt_nmax with "Htrinv H") as ">(H & %)" ; first done.
-    wp_apply (machine_int_add_spec n1 n2 with "[] [H Post]") .
-    {
-      iPureIntro. unfold min_int in *. lia.
-    }
-    {
-      iNext ; iIntros "%". iApply "Post". iFrame "H".
-    }
+    iIntros "#Htrinv" (Φ) "!# ([% H1] & [% H2]) Post".
+    iAssert (TR (Z.to_nat (`n1+`n2))) with "[H1 H2]" as "H".
+    { rewrite Z2Nat.inj_add // TR_plus. iFrame. }
+    iDestruct (TR_lt_nmax with "Htrinv H") as ">(H & Hnmax)" ; [done|].
+    iDestruct "Hnmax" as %Hnmax.
+    assert (`n1 + `n2 < max_mach_int).
+    { rewrite -(Nat2Z.id nmax) in Hnmax. apply Z2Nat.inj_lt in Hnmax; lia. }
+    assert (bool_decide (mach_int_bounded (`n1 + `n2))).
+    { apply bool_decide_pack. split; [|done].
+      (* FIXME : why isn't lia able to do this directly? *)
+      trans 0. unfold min_mach_int; lia. lia. }
+    wp_op.
+    { by rewrite /bin_op_eval /= /to_mach_int /mach_int_bounded decide_left. }
+    iApply "Post". iIntros "{$H} /= !%". lia.
   Qed.
 
 End clock_int.
@@ -48,54 +52,62 @@ Section snapclock_int.
 
   Context `{timeReceiptHeapG Σ}.
   Context (nmax : nat).
-  Context `(nmax ≤ max_int).
+  Context `(nmax ≤ max_mach_int).
 
-  Definition is_snapclock_int (n : nat) : iProp Σ :=
-    TRdup n.
+  Definition is_snapclock_int (n : Z) : iProp Σ :=
+    (⌜0 ≤ n⌝ ∗ TRdup (Z.to_nat n))%I.
 
   (* Snapclock integers are persistent (in particular they are duplicable): *)
-  Lemma snapclock_int_persistent (n : nat) :
+  Lemma snapclock_int_persistent (n : Z) :
     Persistent (is_snapclock_int n).
   Proof. exact _. Qed.
 
   (* Snapclock integers support incrementation: *)
-  Lemma snapclock_int_incr_spec n1 :
+  Lemma snapclock_int_incr_spec (n1 : mach_int) :
     TR_invariant nmax -∗
-    {{{ is_snapclock_int n1 }}}
-    tick #() ;; machine_int_add #n1 #1
-    {{{ RET #(n1+1) ; is_snapclock_int (n1+1) }}}.
+    {{{ is_snapclock_int (`n1) }}}
+    tick #() ;; #n1 + #mach_int_1
+    {{{ H, RET #(LitMachInt ((`n1+1) ↾ H)) ; is_snapclock_int (`n1+1) }}}.
   Proof.
-    iIntros "#Htrinv" (Φ) "!# H1 Post".
+    iIntros "#Htrinv" (Φ) "!# [% H1] Post".
     wp_apply (tick_spec_simple nmax #() with "Htrinv H1"). iIntros "(_ & H)".
-    iDestruct (TRdup_lt_nmax with "Htrinv H") as ">(H & %)" ; first done.
-    wp_seq.
-    wp_apply (machine_int_add_spec n1 1 with "[] [H Post]") .
-    {
-      iPureIntro. unfold min_int in *. lia.
-    }
-    {
-      iNext ; iIntros "%". iApply "Post". iFrame "H".
-    }
+    iDestruct (TRdup_lt_nmax with "Htrinv H") as ">(H & Hnmax)" ; first done.
+    iDestruct "Hnmax" as %Hnmax. wp_seq.
+    assert (`n1 + 1 < max_mach_int).
+    { rewrite -(Nat2Z.id nmax) (_:1%nat = Z.to_nat 1) // -Z2Nat.inj_add // in Hnmax.
+      apply Z2Nat.inj_lt in Hnmax; lia. }
+    assert (bool_decide (mach_int_bounded (`n1 + 1))).
+    { apply bool_decide_pack. split; [|done].
+      (* FIXME : why isn't lia able to do this directly? *)
+      trans 0. unfold min_mach_int; lia. lia. }
+    wp_op.
+    { by rewrite /bin_op_eval /= /to_mach_int /mach_int_bounded decide_left. }
+    iApply "Post". iSplit. auto with lia.
+    by rewrite Z2Nat.inj_add //.
   Qed.
 
   (* Snapclock integers also support a limited form of addition: *)
-  Lemma snapclock_int_add_spec n1 n2 m :
+  Lemma snapclock_int_add_spec (n1 n2 : mach_int) (m : Z) :
     TR_invariant nmax -∗
-    {{{ is_snapclock_int n1 ∗ is_snapclock_int n2
-      ∗ is_snapclock_int m ∗ ⌜n1+n2 ≤ m⌝ }}}
-    machine_int_add #n1 #n2
-    {{{ RET #(n1+n2) ; is_snapclock_int (n1+n2) }}}.
+    {{{ is_snapclock_int (`n1) ∗ is_snapclock_int (`n2)
+      ∗ is_snapclock_int m ∗ ⌜`n1+`n2 ≤ m⌝ }}}
+    #n1 + #n2
+    {{{ H, RET #(LitMachInt ((`n1+`n2) ↾ H)) ; is_snapclock_int (`n1+`n2) }}}.
   Proof.
-    iIntros "#Htrinv" (Φ) "!# (_ & _ & Hm & %) Post".
-    iDestruct (TRdup_lt_nmax with "Htrinv Hm") as ">(Hm & %)" ; first done.
-    iDestruct (TRdup_weaken m (n1 + n2) with "Hm") as "H" ; first lia.
-    wp_apply (machine_int_add_spec n1 n2 with "[] [H Post]") .
-    {
-      iPureIntro. unfold min_int in *. lia.
-    }
-    {
-      iNext ; iIntros "%". iApply "Post". iFrame "H".
-    }
+    iIntros "#Htrinv" (Φ) "!# ([% _] & [% _] & [% Hm] & %) Post".
+    iDestruct (TRdup_lt_nmax with "Htrinv Hm") as ">(Hm & Hnmax)" ; first done.
+    iDestruct "Hnmax" as %Hnmax.
+    assert (m < max_mach_int).
+    { rewrite -(Nat2Z.id nmax) in Hnmax. apply Z2Nat.inj_lt in Hnmax; lia. }
+    iDestruct (TRdup_weaken (Z.to_nat m) (Z.to_nat (`n1 + `n2)) with "Hm") as "H".
+    { apply Z2Nat.inj_le; lia. }
+    assert (bool_decide (mach_int_bounded (`n1 + `n2))).
+    { apply bool_decide_pack. split; [|lia].
+      (* FIXME : why isn't lia able to do this directly? *)
+      trans 0. unfold min_mach_int; lia. lia. }
+    wp_op.
+    { by rewrite /bin_op_eval /= /to_mach_int /mach_int_bounded decide_left. }
+    iApply "Post". iSplit; [|done]. auto with lia.
   Qed.
 
 End snapclock_int.
