theories/Reduction.v
@@ -1,5 +1,5 @@
-From iris.heap_lang Require Import lang notation.
-From iris.heap_lang Require Import adequacy.
+From iris_time.heap_lang Require Import lang notation.
+From iris_time.heap_lang Require Import adequacy.
 From stdpp Require Import relations fin_maps gmap.
 
 From iris_time Require Import Misc Tactics.
@@ -20,18 +20,19 @@ Implicit Type m n : nat.
 Section Reduction.
 
   Definition bounded_time e σ m : Prop :=
-    ∀ t2 σ2 n, nsteps step n ([e], σ) (t2, σ2) → (n ≤ m)%nat.
+    ∀ t2 σ2 n, nsteps erased_step n ([e], σ) (t2, σ2) → (n ≤ m)%nat.
 
   Inductive prim_exec (e1 : expr) (σ1 : state) : expr → state → list expr → Prop :=
   | prim_exec_nil :
       prim_exec e1 σ1 e1 σ1 []
-  | prim_exec_cons (e2 : expr) (σ2 : state) (efs2 : list expr) e3 σ3 efs3 :
-      prim_step e1 σ1 e2 σ2 efs2 →
+  | prim_exec_cons (κ : list Empty_set)
+                   (e2 : expr) (σ2 : state) (efs2 : list expr) e3 σ3 efs3 :
+      prim_step e1 σ1 κ e2 σ2 efs2 →
       prim_exec e2 σ2 e3 σ3 efs3 →
       prim_exec e1 σ1 e3 σ3 (efs2 ++ efs3).
 
-  Lemma prim_exec_cons_nofork e1 σ1 e2 σ2 e3 σ3 efs3 :
-    prim_step e1 σ1 e2 σ2 []   →
+  Lemma prim_exec_cons_nofork e1 σ1 κ e2 σ2 e3 σ3 efs3 :
+    prim_step e1 σ1 κ e2 σ2 []   →
     prim_exec e2 σ2 e3 σ3 efs3 →
     prim_exec e1 σ1 e3 σ3 efs3.
   Proof.
@@ -54,8 +55,8 @@ Section Reduction.
     intros. change efs3 with ([] ++ efs3). by eapply prim_exec_transitive.
   Qed.
 
-  Lemma thread_pool_grows_after_step t1 σ1 t2 σ2 :
-    step (t1, σ1) (t2, σ2) →
+  Lemma thread_pool_grows_after_step t1 σ1 κ t2 σ2 :
+    step (t1, σ1) κ (t2, σ2) →
     (length t1 ≤ length t2)%nat.
   Proof.
     intros [e1 σ1_ e2 σ2_ efs t t' E1 E2 Hstep] ;
@@ -63,14 +64,14 @@ Section Reduction.
     repeat rewrite ? app_length ? cons_length. lia.
   Qed.
   Lemma thread_pool_grows_after_exec t1 σ1 t2 σ2 :
-    rtc step (t1, σ1) (t2, σ2) →
+    rtc erased_step (t1, σ1) (t2, σ2) →
     (length t1 ≤ length t2)%nat.
   Proof.
     make_eq (t1, σ1) as config1 E1.
     make_eq (t2, σ2) as config2 E2.
     intros Hsteps.
     revert t1 σ1 E1 ;
-    induction Hsteps as [ config | config1 (t3, σ3) config2 Hstep _ IHsteps ] ;
+    induction Hsteps as [ config | config1 (t3, σ3) config2 [κ Hstep] _ IHsteps ] ;
     intros t1 σ1 E1.
     - destruct E2 ; injection E1 as -> ->.
       done.
@@ -79,8 +80,8 @@ Section Reduction.
       + by eapply thread_pool_grows_after_step.
       + by eapply IHsteps.
   Qed.
-  Lemma thread_pool_is_cons_after_step t1 σ1 t2 σ2 :
-    step (t1, σ1) (t2, σ2) →
+  Lemma thread_pool_is_cons_after_step t1 σ1 κ t2 σ2 :
+    step (t1, σ1) κ (t2, σ2) →
     ∃ e2 t2', t2 = e2 :: t2'.
   Proof.
     intros Hstep.
@@ -94,7 +95,7 @@ Section Reduction.
     - eauto.
   Qed.
   Lemma thread_pool_is_cons_after_exec e1 t1' σ1 t2 σ2 :
-    rtc step (e1 :: t1', σ1) (t2, σ2) →
+    rtc erased_step (e1 :: t1', σ1) (t2, σ2) →
     ∃ e2 t2', t2 = e2 :: t2'.
   Proof.
     destruct t2.
@@ -102,10 +103,10 @@ Section Reduction.
     - eauto.
   Qed.
 
-  Lemma step_insert_in_thread_pool (n : nat) t t1 σ1 t2 σ2 :
+  Lemma step_insert_in_thread_pool (n : nat) t t1 σ1 κ t2 σ2 :
     (n ≤ length t1)%nat →
-    step (t1, σ1) (t2, σ2) →
-    step (take n t1 ++ t ++ drop n t1, σ1) (take n t2 ++ t ++ drop n t2, σ2).
+    step (t1, σ1) κ (t2, σ2) →
+    step (take n t1 ++ t ++ drop n t1, σ1) κ (take n t2 ++ t ++ drop n t2, σ2).
   Proof.
     intros I Hstep.
     destruct Hstep as [e1 σ1_ e2 σ2_ efs ta tb E1 E2 Hprimstep] ; simpl in * ;
@@ -129,26 +130,26 @@ Section Reduction.
   Qed.
   Lemma exec_insert_in_thread_pool (n : nat) t t1 σ1 t2 σ2 :
     (n ≤ length t1)%nat →
-    rtc step (t1, σ1) (t2, σ2) →
-    rtc step (take n t1 ++ t ++ drop n t1, σ1) (take n t2 ++ t ++ drop n t2, σ2).
+    rtc erased_step (t1, σ1) (t2, σ2) →
+    rtc erased_step (take n t1 ++ t ++ drop n t1, σ1) (take n t2 ++ t ++ drop n t2, σ2).
   Proof.
     make_eq (t1, σ1) as config1 E1.
     make_eq (t2, σ2) as config2 E2.
     intros I H.
     revert t1 σ1 E1 I ;
-    induction H as [ config | config1 (t3, σ3) config2 Hstep _ IHsteps ] ;
+    induction H as [ config | config1 (t3, σ3) config2 [κ Hstep] _ IHsteps ] ;
     intros t1 σ1 E1 I.
     - destruct E2 ; injection E1 as -> ->.
       apply rtc_refl.
     - destruct E2, E1.
       eapply rtc_l.
-      + by eapply step_insert_in_thread_pool.
+      + exists κ. by eapply step_insert_in_thread_pool.
       + by eapply IHsteps, le_trans, thread_pool_grows_after_step.
   Qed.
   Lemma exec_frame_thread_pool t1 σ1 t2 σ2 ta tb :
-    rtc step (t1, σ1) (t2, σ2) →
+    rtc erased_step (t1, σ1) (t2, σ2) →
     let n := length t1 in
-    rtc step (ta ++ t1 ++ tb, σ1) (ta ++ take n t2 ++ tb ++ drop n t2, σ2).
+    rtc erased_step (ta ++ t1 ++ tb, σ1) (ta ++ take n t2 ++ tb ++ drop n t2, σ2).
   Proof.
     intros Hsteps n.
     replace (t1 ++ tb) with (take n t1 ++ tb ++ drop n t1)
@@ -156,29 +157,30 @@ Section Reduction.
     apply (exec_insert_in_thread_pool 0 ta), (exec_insert_in_thread_pool n tb) ; first lia ; done.
   Qed.
   Lemma exec_frame_singleton_thread_pool e1 σ1 e2 t2 σ2 t t' :
-    rtc step ([e1], σ1) (e2 :: t2, σ2) →
-    rtc step (t ++ e1 :: t', σ1) (t ++ e2 :: t' ++ t2, σ2).
+    rtc erased_step ([e1], σ1) (e2 :: t2, σ2) →
+    rtc erased_step (t ++ e1 :: t', σ1) (t ++ e2 :: t' ++ t2, σ2).
   Proof.
     change (e1 :: t') with ([e1] ++ t').
     apply exec_frame_thread_pool.
   Qed.
 
-  Lemma prim_step_step e1 σ1 e2 σ2 efs :
-    prim_step e1 σ1 e2 σ2 efs →
-    step ([e1], σ1) (e2 :: efs, σ2).
+  Lemma prim_step_step e1 σ1 κ e2 σ2 efs :
+    prim_step e1 σ1 κ e2 σ2 efs →
+    step ([e1], σ1) κ (e2 :: efs, σ2).
   Proof.
     intros. by eapply step_atomic with _ _ _ _ _ [] [].
   Qed.
   Lemma prim_exec_exec e1 σ1 e2 σ2 efs :
     prim_exec e1 σ1 e2 σ2 efs →
-    rtc step ([e1], σ1) (e2 :: efs, σ2).
+    rtc erased_step ([e1], σ1) (e2 :: efs, σ2).
   Proof.
+    unfold erased_step.
     induction 1 ; econstructor ; eauto using prim_step_step, (exec_frame_singleton_thread_pool _ _ _ _ _ []).
   Qed.
 
-  Lemma prim_step_fill K e1 σ1 e2 σ2 efs :
-    prim_step e1 σ1 e2 σ2 efs →
-    prim_step (fill K e1) σ1 (fill K e2) σ2 efs.
+  Lemma prim_step_fill K e1 σ1 κ e2 σ2 efs :
+    prim_step e1 σ1 κ e2 σ2 efs →
+    prim_step (fill K e1) σ1 κ (fill K e2) σ2 efs.
   Proof.
     intros [ K' e1' e2' -> -> Hheadstep ].
     rewrite - 2! fill_app.
@@ -199,9 +201,9 @@ Section Reduction.
     intros <- <-. apply prim_exec_fill.
   Qed.
 
-  Lemma step_fill K e1 t1' σ1 e2 t2' σ2 :
-    step (e1 :: t1', σ1) (e2 :: t2', σ2) →
-    step (fill K e1 :: t1', σ1) (fill K e2 :: t2', σ2).
+  Lemma step_fill K e1 t1' σ1 κ e2 t2' σ2 :
+    step (e1 :: t1', σ1) κ (e2 :: t2', σ2) →
+    step (fill K e1 :: t1', σ1) κ (fill K e2 :: t2', σ2).
   Proof.
     intros Hstep.
     destruct Hstep as [ e1' ? e2' ? efs ta tb E1 E2 ] ;
@@ -211,14 +213,14 @@ Section Reduction.
     - by eapply step_atomic with _ _ _ _ _ (fill K e2 :: ta) tb.
   Qed.
   Lemma exec_fill K e1 t1' σ1 e2 t2' σ2 :
-    rtc step (e1 :: t1', σ1) (e2 :: t2', σ2) →
-    rtc step (fill K e1 :: t1', σ1) (fill K e2 :: t2', σ2).
+    rtc erased_step (e1 :: t1', σ1) (e2 :: t2', σ2) →
+    rtc erased_step (fill K e1 :: t1', σ1) (fill K e2 :: t2', σ2).
   Proof.
     make_eq (e1 :: t1', σ1) as config1 E1.
     make_eq (e2 :: t2', σ2) as config2 E2.
     intros Hsteps.
     revert e1 t1' σ1 E1 ;
-    induction Hsteps as [ config | config1 (t3, σ3) config2 Hstep _ IHsteps ] ;
+    induction Hsteps as [ config | config1 (t3, σ3) config2 [κ Hstep] _ IHsteps ] ;
     intros e1 t1' σ1 E1.
     - destruct E2 ; injection E1 as -> -> ->.
       apply rtc_refl.
@@ -226,7 +228,7 @@ Section Reduction.
       assert (∃ e3 t3', t3 = e3 :: t3') as (e3 & t3' & ->)
         by by eapply thread_pool_is_cons_after_step.
       eapply rtc_l.
-      + by apply step_fill.
+      + exists κ. by apply step_fill.
       + by apply IHsteps.
   Qed.
 
@@ -234,100 +236,12 @@ Section Reduction.
     reducible e σ →
     reducible (fill K e) σ.
   Proof.
-    intros (e' & σ' & efs & Hstep).
-    eexists _, _, _.
+    intros (κ & e' & σ' & efs & Hstep).
+    eexists _, _, _, _.
     by apply prim_step_fill.
   Qed.
 
 End Reduction.
-
-
-
-(*
- * Closed expressions
- *)
-
-Section Closed.
-
-  Lemma is_closed_fill_inv xs K e :
-    is_closed xs (fill K e) →
-    is_closed xs e.
-  Proof.
-    replace K with (rev (rev K)) by apply rev_involutive.
-    induction (rev K) as [ | [] revK' ] ; first done ;
-    rewrite /= fill_app /= ; naive_solver.
-  Qed.
-
-  Lemma is_closed_fill xs K e :
-    is_closed xs e →
-    (∃ e0, is_closed xs (fill K e0)) →
-    is_closed xs (fill K e).
-  Proof.
-    intros He [e0 HK] ; revert HK.
-    replace K with (rev (rev K)) by apply rev_involutive.
-    induction (rev K) as [ | [] revK' ] ; first done ;
-    rewrite /= !fill_app /= ; naive_solver.
-  Qed.
-
-  Lemma is_closed_head_step xs e1 σ1 e2 σ2 efs :
-    is_closed xs e1 →
-    head_step e1 σ1 e2 σ2 efs →
-    is_closed xs e2 ∧ Forall (is_closed xs) efs.
-  Proof.
-    intros Hclosed Hstep.
-    destruct Hstep as
-      [ (* BetaS *) f x e1 e2 v2 e' σ  Hval_e2 Hclosed_e1 ->
-      | | | | | | | | | | | | | | | ] ;
-    (split ; last auto) ;
-    rewrite_into_values ;
-    try (by apply is_closed_of_val) ;
-    try naive_solver.
-    (* BetaS f x e1 e2 v2 e' σ : *)
-    - apply is_closed_do_subst', is_closed_do_subst' ; try naive_solver. by apply is_closed_of_val.
-  Qed.
-  Lemma is_closed_prim_step xs e1 σ1 e2 σ2 efs :
-    is_closed xs e1 →
-    prim_step e1 σ1 e2 σ2 efs →
-    is_closed xs e2 ∧ Forall (is_closed xs) efs.
-  Proof.
-    intros HKe1' [K e1' e2' -> -> Hstep] ; simpl in *. 
-    eapply is_closed_head_step in Hstep as [??] ; last by eapply is_closed_fill_inv.
-    eauto using is_closed_fill.
-  Qed.
-  Lemma is_closed_step xs t1 σ1 t2 σ2 :
-    Forall (is_closed xs) t1 →
-    step (t1, σ1) (t2, σ2) →
-    Forall (is_closed xs) t2.
-  Proof.
-    intros Hclosed Hstep.
-    destruct Hstep as [e1 σ1_ e2 σ2_ efs tl tr E1 E2 Hstep] ;
-    injection E1 as -> <- ; injection E2 as -> <- ;
-    simpl.
-    rewrite -> ? Forall_app, ? Forall_cons in Hclosed. repeat (destruct Hclosed as [? Hclosed]).
-    eapply is_closed_prim_step in Hstep as [??] ; last eassumption.
-    repeat (rewrite ? Forall_app ? Forall_cons ; repeat split) ; assumption.
-  Qed.
-  Lemma is_closed_exec xs t1 σ1 t2 σ2 :
-    Forall (is_closed xs) t1 →
-    rtc step (t1, σ1) (t2, σ2) →
-    Forall (is_closed xs) t2.
-  Proof.
-    make_eq (t1, σ1) as config1 E1.
-    make_eq (t2, σ2) as config2 E2.
-    intros Hclosed Hsteps.
-    revert t1 σ1 E1 Hclosed ;
-    induction Hsteps as [ config | config1 (t3, σ3) config2 Hstep _ IHsteps ] ;
-    intros t1 σ1 E1 Hclosed.
-    - destruct E2 ; injection E1 as -> _.
-      done.
-    - destruct E2, E1.
-      eapply is_closed_step in Hstep ; last done.
-      by eapply IHsteps.
-  Qed.
-
-End Closed.
-
-
 
 (*
  * Fresh locations
@@ -335,25 +249,25 @@ End Closed.
 
 Section FreshLocation.
 
-  Lemma loc_fresh_in_dom_head_step ℓ e1 σ1 e2 σ2 efs :
+  Lemma loc_fresh_in_dom_head_step ℓ e1 σ1 κ e2 σ2 efs :
     σ2 !! ℓ = None →
-    head_step e1 σ1 e2 σ2 efs →
+    head_step e1 σ1 κ e2 σ2 efs →
     σ1 !! ℓ = None.
   Proof.
     intros Hℓ H ; destruct H ; try done ;
     by apply lookup_insert_None in Hℓ as [ Hℓ _ ].
   Qed.
-  Lemma loc_fresh_in_dom_prim_step ℓ e1 σ1 e2 σ2 efs :
+  Lemma loc_fresh_in_dom_prim_step ℓ e1 σ1 κ e2 σ2 efs :
     σ2 !! ℓ = None →
-    prim_step e1 σ1 e2 σ2 efs →
+    prim_step e1 σ1 κ e2 σ2 efs →
     σ1 !! ℓ = None.
   Proof.
     intros Hℓ H ; destruct H ;
     by eapply loc_fresh_in_dom_head_step.
   Qed.
-  Lemma loc_fresh_in_dom_step ℓ t1 σ1 t2 σ2 :
+  Lemma loc_fresh_in_dom_step ℓ t1 σ1 κ t2 σ2 :
     σ2 !! ℓ = None →
-    step (t1, σ1) (t2, σ2) →
+    step (t1, σ1) κ (t2, σ2) →
     σ1 !! ℓ = None.
   Proof.
     intros Hℓ H ; destruct H as [ ? ? ? ? ? ? ? E1 E2 Hstep ] ;
@@ -362,26 +276,26 @@ Section FreshLocation.
   Qed.
   Lemma loc_fresh_in_dom_nsteps ℓ m t1 σ1 t2 σ2 :
     σ2 !! ℓ = None →
-    nsteps step m (t1, σ1) (t2, σ2) →
+    nsteps erased_step m (t1, σ1) (t2, σ2) →
     σ1 !! ℓ = None.
   Proof.
     make_eq (t1, σ1) as config1 E1.
     make_eq (t2, σ2) as config2 E2.
     intros Hℓ H.
     revert t1 σ1 E1 ;
-    induction H as [ config | _ config1 (t3, σ3) config2 Hstep _ IHnsteps ] ;
+    induction H as [ config | ? config1 (t3, σ3) config2 [κ Hstep] _ IHnsteps ] ;
     intros t1 σ1 E1.
     - destruct E2 ; injection E1 as -> ->.
       done.
     - destruct E2, E1.
       specialize (IHnsteps eq_refl t3 σ3 eq_refl).
-      eapply loc_fresh_in_dom_step ; eassumption.
+      eapply loc_fresh_in_dom_step; eassumption.
   Qed.
 
   Fixpoint loc_set_of_expr e : gset loc :=
     match e with
-    | Lit (LitLoc l) => {[ l ]}
-    | Lit _ | Var _ => empty
+    | Val v => loc_set_of_val v
+    | Var _ => empty
     | Rec _ _ e
     | UnOp _ e | Fst e | Snd e | InjL e | InjR e | Fork e | Alloc e | Load e =>
        loc_set_of_expr e
@@ -389,12 +303,20 @@ Section FreshLocation.
        loc_set_of_expr e1 ∪ loc_set_of_expr e2
     | If e0 e1 e2 | Case e0 e1 e2 | CAS e0 e1 e2 =>
        loc_set_of_expr e0 ∪ loc_set_of_expr e1 ∪ loc_set_of_expr e2
+    end
+  with loc_set_of_val v : gset loc :=
+    match v with
+    | LitV (LitLoc l) => {[ l ]}
+    | LitV _ => empty
+    | RecV _ _ e => loc_set_of_expr e
+    | InjLV v | InjRV v => loc_set_of_val v
+    | PairV v1 v2 => loc_set_of_val v1 ∪ loc_set_of_val v2
     end.
 
   Fixpoint loc_fresh_in_expr (ℓ : loc) e : bool :=
     match e with
-    | Lit (LitLoc l) => bool_decide (ℓ ≠ l)
-    | Lit _ | Var _ => true
+    | Val v => loc_fresh_in_val (ℓ : loc) v
+    | Var _ => true
     | Rec _ _ e
     | UnOp _ e | Fst e | Snd e | InjL e | InjR e | Fork e | Alloc e | Load e =>
        loc_fresh_in_expr ℓ e
@@ -402,20 +324,31 @@ Section FreshLocation.
        loc_fresh_in_expr ℓ e1 && loc_fresh_in_expr ℓ e2
     | If e0 e1 e2 | Case e0 e1 e2 | CAS e0 e1 e2 =>
        loc_fresh_in_expr ℓ e0 && loc_fresh_in_expr ℓ e1 && loc_fresh_in_expr ℓ e2
+    end
+  with loc_fresh_in_val (ℓ : loc) v : bool :=
+    match v with
+    | LitV (LitLoc l) => bool_decide (ℓ ≠ l)
+    | LitV _ => true
+    | RecV _ _ e => loc_fresh_in_expr ℓ e
+    | InjLV v | InjRV v => loc_fresh_in_val ℓ v
+    | PairV v1 v2 => loc_fresh_in_val ℓ v1 && loc_fresh_in_val ℓ v2
     end.
 
-  Lemma loc_not_in_set_is_fresh (ℓ : loc) e :
+  Lemma loc_not_in_set_is_fresh_in_expr (ℓ : loc) e :
     ℓ ∉ loc_set_of_expr e →
-    loc_fresh_in_expr ℓ e.
+    loc_fresh_in_expr ℓ e
+  with loc_not_in_set_is_fresh_in_val (ℓ : loc) v :
+    ℓ ∉ loc_set_of_val v →
+    loc_fresh_in_val ℓ v.
   Proof.
-    (* this works but is slow: *)
-(*     induction e ; try set_solver. *)
-    (* fast manual proof: *)
-    induction e ; simpl ;
-    intros Hnotin ; repeat (apply not_elem_of_union in Hnotin as [Hnotin ?]) ;
-    auto 10.
-    (* only remaining case: e = Lit l *)
-    case_match ; set_solver.
+    - destruct e; simpl; intros Hnotin ;
+        repeat (apply not_elem_of_union in Hnotin as [Hnotin ?]) ;
+        auto 10.
+    - destruct v as [[]| | | |]; simpl; intros Hnotin ;
+        repeat (apply not_elem_of_union in Hnotin as [Hnotin ?]) ;
+        auto 10.
+      (* only remaining case: v = LitV l *)
+      apply bool_decide_pack. set_solver.
   Qed.
 
   Lemma loc_fresh_in_expr_fill_inv (ℓ : loc) K e :
@@ -440,7 +373,8 @@ Section ActiveItem.
 
   Definition ectx_item_is_active (Ki : ectx_item) : bool :=
     match Ki with
-    | AppLCtx _ | UnOpCtx _ | BinOpLCtx _ _ | IfCtx _ _ | FstCtx | SndCtx
+    | AppLCtx _ | UnOpCtx _ | BinOpLCtx _ _ | IfCtx _ _
+    | PairLCtx _ | FstCtx | SndCtx | InjLCtx | InjRCtx
     | CaseCtx _ _ | AllocCtx | LoadCtx | StoreLCtx _ | CasLCtx _ _ | FaaLCtx _ => true
     | _ => false
     end.
@@ -463,7 +397,7 @@ Section ActiveItem.
         let K0 := fresh "K0" in
         destruct (IH eq_refl) as (K0 & ? & -> & ? & ?) ; clear IH ;
         lazymatch goal with |- to_val ?e = None → _ =>
-          reshape_expr e ltac:(fun K1 _ =>
+          reshape_expr false e ltac:(fun K1 _ =>
             eexists (K0 ++ K1), _ ; split ; [|split] ;
             [ by erewrite fill_app | assumption | assumption ]
           )
@@ -474,7 +408,7 @@ Section ActiveItem.
   Local Ltac maximal_ectx_empty :=
     eexists [], _ ; split ; [|split] ;
     [ reflexivity | assumption | ] ;
-    intros [] ; try discriminate ; inversion 1 ; rewrite to_of_val ; eauto.
+    intros [] ; inversion 1 ; eauto.
 
   Lemma not_val_maximal_ectx e :
     to_val e = None →
@@ -492,12 +426,12 @@ Section ActiveItem.
     (* we perform rewriting for each immediate sub-redex of e (we read e again
      * after each iteration because previous rewritings reveal new contexts): *)
     repeat (lazymatch type of Hsubterms with immediate_sub_redexes_are_values ?e =>
-        reshape_expr e ltac:(fun K e1 =>
+        reshape_expr false e ltac:(fun K e1 =>
           (* we are only interested in contexts of depth 1; moreover, for
            * termination purposes, we do nothing when the hole e1 is already
            * a value: *)
           lazymatch constr:(pair K e1) with
-          | pair _ (of_val ?v) =>
+          | pair _ (Val ?v) =>
               fail
           | pair [ ?Ki ] _ =>
               let v := fresh "v" in
@@ -507,12 +441,12 @@ Section ActiveItem.
     end).
 
   Local Ltac exhibit_active_item :=
-    lazymatch goal with |- exists ki v, ?e = fill_item ki (of_val v) ∧ Is_true (ectx_item_is_active ki) =>
-        reshape_expr e ltac:(fun K e1 =>
+    lazymatch goal with |- exists ki v, ?e = fill_item ki (Val v) ∧ Is_true (ectx_item_is_active ki) =>
+        reshape_expr false e ltac:(fun K e1 =>
           (* we are only interested in contexts of depth 1; moreover, we are
            * supposed to get a value in the hole: *)
           lazymatch constr:(pair K e1) with
-          | pair [ ?Ki ] (of_val ?v) =>
+          | pair [ ?Ki ] (Val ?v) =>
               (* we try to conclude with that context item (if it is not active,
                * then the proof will fail, thus we do not need to test it ourself): *)
               by exists Ki, v
@@ -521,41 +455,42 @@ Section ActiveItem.
     end.
 
   Lemma sub_redexes_values_active_item e0 :
-    is_closed [] e0 →
     to_val e0 = None →
     immediate_sub_redexes_are_values e0 →
-      (∃ e1, e0 = Fork e1)
+      (∃ x, e0 = Var x)
+    ∨ (∃ e1, e0 = Fork e1)
+    ∨ (∃ f x e1, e0 = Rec f x e1)
     ∨ (∃ (ki : ectx_item) (v : val),
         e0 = fill_item ki v
       ∧ ectx_item_is_active ki).
   Proof.
-    intros Hclosed Hnotval Hsubterms.
+    intros Hnotval Hsubterms.
     destruct e0 ;
       rewrite_immediate_sub_redexes_into_values Hsubterms ;
       (* most cases are solved by exhibiting a solution: *)
-      try (right ; exhibit_active_item) ;
+      try (right ; right; right; exhibit_active_item) ;
       (* some cases contradict the assumption that e0 is not a value: *)
-      rewrite /= ? to_of_val in Hnotval ;
       try discriminate Hnotval.
     (* remaining cases : *)
-    (* Var: contradict the closedness assumption *)
-    - contradiction Hclosed.
-    (* Rec: contradict either closedness or the fact that e0 is not a value *)
-    - case_match ; [ discriminate Hnotval | contradiction Hclosed ].
-    (* Fork: the only really special case *)
-    - left. eauto.
+    (* Var *)
+    - eauto.
+    (* Rec *)
+    - eauto 10.
+    (* Fork *)
+    - eauto 10.
   Qed.
 
   Lemma not_val_fill_active_item e :
-    is_closed [] e →
     to_val e = None →
-      (∃ K e1, e = fill K (Fork e1))
+      (∃ K x, e = fill K (Var x))
+    ∨ (∃ K e1, e = fill K (Fork e1))
+    ∨ (∃ K f x e1, e = fill K (Rec f x e1))
     ∨ (∃ K ki v, e = fill K (fill_item ki v) ∧ ectx_item_is_active ki).
   Proof.
-    intros Hclosed (K & e0 & -> & Hnotval & Hsubterms) % not_val_maximal_ectx.
-    apply is_closed_fill_inv in Hclosed.
+    intros (K & e0 & -> & Hnotval & Hsubterms) % not_val_maximal_ectx.
     apply sub_redexes_values_active_item in Hsubterms
-      as [ [e1 ->] | (ki & v & -> & Hactive) ] ; naive_solver.
+      as [ [x ->] | [[e1 ->] | [(f & x & e1 & ->) | (ki & v & -> & Hactive)]] ];
+    naive_solver.
   Qed.
 
   Lemma active_item_not_val ki e :
@@ -571,13 +506,13 @@ Section ActiveItem.
   Proof.
     destruct ki ; try contradiction ; intros _ ;
     intros [] ? ; try discriminate 1 ;
-    injection 1 ; repeat (intros <- || intros _) ; rewrite to_of_val ; eauto.
+    injection 1 ; repeat (intros <- || intros _) ; eauto.
   Qed.
 
-  Lemma active_item_prim_step_is_head_step ki v σ1 e2 σ2 efs :
+  Lemma active_item_prim_step_is_head_step ki v σ1 κ e2 σ2 efs :
     ectx_item_is_active ki →
-    prim_step (fill_item ki v) σ1 e2 σ2 efs →
-    head_step (fill_item ki v) σ1 e2 σ2 efs.
+    prim_step (fill_item ki v) σ1 κ e2 σ2 efs →
+    head_step (fill_item ki v) σ1 κ e2 σ2 efs.
   Proof.
     intros Hactive Hstep.
     destruct Hstep as [K' e1' e2' E1 E2 Hheadstep] ; simpl in *.
@@ -661,7 +596,7 @@ Section Safety.
   Lemma safe_exec e1 σ1 t2 e2 σ2 :
     e2 ∈ t2 →
     safe e1 σ1 →
-    rtc step ([e1], σ1) (t2, σ2) →
+    rtc erased_step ([e1], σ1) (t2, σ2) →
     safe e2 σ2.
   Proof.
     intros E2 Hsafe1 Hsteps1to2.
@@ -677,7 +612,7 @@ Section Safety.
   Lemma not_safe_exec e1 σ1 t2 e2 σ2 :
     e2 ∈ t2 →
     ¬ safe e2 σ2 →
-    rtc step ([e1], σ1) (t2, σ2) →
+    rtc erased_step ([e1], σ1) (t2, σ2) →
     ¬ safe e1 σ1.
   Proof.
     eauto 10 using safe_exec.
@@ -685,24 +620,24 @@ Section Safety.
 
   Lemma safe_exec_nofork e1 σ1 e2 σ2 :
     safe e1 σ1 →
-    rtc step ([e1], σ1) ([e2], σ2) →
+    rtc erased_step ([e1], σ1) ([e2], σ2) →
     safe e2 σ2.
   Proof.
     intros. eapply safe_exec ; [ constructor | eassumption | eassumption ].
   Qed.
 
-  Lemma safe_prim_step e1 σ1 e2 σ2 efs :
+  Lemma safe_prim_step e1 σ1 κ e2 σ2 efs :
     safe e1 σ1 →
-    prim_step e1 σ1 e2 σ2 efs →
+    prim_step e1 σ1 κ e2 σ2 efs →
     safe e2 σ2.
   Proof.
     intros. eapply safe_exec ; [ constructor | eassumption | ].
-    eapply rtc_l, rtc_refl. apply prim_step_step. eassumption.
+    eapply rtc_l, rtc_refl. exists κ. apply prim_step_step. eassumption.
   Qed.
 
-  Lemma not_safe_prim_step e1 σ1 e2 σ2 efs :
+  Lemma not_safe_prim_step e1 σ1 κ e2 σ2 efs :
     ¬ safe e2 σ2 →
-    prim_step e1 σ1 e2 σ2 efs →
+    prim_step e1 σ1 κ e2 σ2 efs →
     ¬ safe e1 σ1.
   Proof.
     eauto using safe_prim_step.
@@ -725,7 +660,7 @@ Section Safety.
     unfold stuck.
     split.
     - by apply fill_not_val.
-    - intros e' σ' efs [K1 e1 e'1 E -> Hstep] ; simpl in *.
+    - intros e' σ' efs κ [K1 e1 e'1 E -> Hstep] ; simpl in *.
       eapply step_by_val in E as HK ; try done ; destruct HK as [K'1 -> ].
       rewrite fill_app in E ; apply fill_inj in E.
       eapply Hirred. econstructor ; [|reflexivity|] ; eassumption.
@@ -743,10 +678,10 @@ Section Safety.
       destruct Hsafe as [ Hval | Hred ].
       + left. by eapply fill_val.
       + destruct (to_val e') eqn:Hnotval ; first by eauto. right.
-        destruct Hred as (_ & σ'' & efs & [ K2 e'2 e''2 Efill _ Hstep ]) ; simpl in *.
+        destruct Hred as (κ & _ & σ'' & efs & [ K2 e'2 e''2 Efill _ Hstep ]) ; simpl in *.
         eapply step_by_val in Efill as Efill' ; try eassumption ; destruct Efill' as [K' ->].
         rewrite fill_app in Efill ; apply fill_inj in Efill as ->.
-        exists (fill K' e''2), σ'', efs.
+        exists κ, (fill K' e''2), σ'', efs.
         by apply Ectx_step'.
     - eapply exec_fill in Hsteps.
       eapply Hsafe ; eauto using elem_of_list_further.
@@ -770,10 +705,10 @@ Section Safety.
   (* n-adequacy: *)
   Record nadequate (s : stuckness) (n : nat) e1 σ1 (φ : val → Prop) : Prop := {
     nadequate_result k t2 σ2 v2 :
-     nsteps step k ([e1], σ1) (of_val v2 :: t2, σ2) → (k ≤ n)%nat → φ v2;
+     nsteps erased_step k ([e1], σ1) (Val v2 :: t2, σ2) → (k ≤ n)%nat → φ v2;
     nadequate_not_stuck k t2 σ2 e2 :
      s = NotStuck →
-     nsteps step k ([e1], σ1) (t2, σ2) →
+     nsteps erased_step k ([e1], σ1) (t2, σ2) →
      (k < n)%nat →
      e2 ∈ t2 → (is_Some (to_val e2) ∨ reducible e2 σ2)
   }.
