theories/Tactics.v
@@ -1,73 +1,9 @@
-From iris.heap_lang Require Export lang tactics.
-
-
-
-(*
- * Tactics for reducing terms
- *)
-
-Ltac simpl_to_of_val :=
-  rewrite /= ? to_of_val //.
-
-Ltac rewrite_into_values :=
-  repeat (lazymatch goal with
-  | H : to_val _ = Some _ |- _ =>
-      eapply of_to_val in H as <-
-  end).
-
-Ltac reshape_expr_ordered b e tac :=
-  let rec go K e :=
-  match e with
-  | _ =>
-      lazymatch b with
-      | false => tac K e
-      | true  => fail
-      end
-  | App ?e1 ?e2 => reshape_val e2 ltac:(fun v2 => go (AppLCtx v2 :: K) e1)
-  | App ?e1 ?e2 => go (AppRCtx e1 :: K) e2
-  | UnOp ?op ?e => go (UnOpCtx op :: K) e
-  | BinOp ?op ?e1 ?e2 =>
-     reshape_val e2 ltac:(fun v2 => go (BinOpLCtx op v2 :: K) e1)
-  | BinOp ?op ?e1 ?e2 => go (BinOpRCtx op e1 :: K) e2
-  | If ?e0 ?e1 ?e2 => go (IfCtx e1 e2 :: K) e0
-  | Pair ?e1 ?e2 => reshape_val e2 ltac:(fun v2 => go (PairLCtx v2 :: K) e1)
-  | Pair ?e1 ?e2 => go (PairRCtx e1 :: K) e2
-  | Fst ?e => go (FstCtx :: K) e
-  | Snd ?e => go (SndCtx :: K) e
-  | InjL ?e => go (InjLCtx :: K) e
-  | InjR ?e => go (InjRCtx :: K) e
-  | Case ?e0 ?e1 ?e2 => go (CaseCtx e1 e2 :: K) e0
-  | Alloc ?e => go (AllocCtx :: K) e
-  | Load ?e => go (LoadCtx :: K) e
-  | Store ?e1 ?e2 => reshape_val e2 ltac:(fun v2 => go (StoreLCtx v2 :: K) e1)
-  | Store ?e1 ?e2 => go (StoreRCtx e1 :: K) e2
-  | CAS ?e0 ?e1 ?e2 => reshape_val e2 ltac:(fun v2 => first
-     [ reshape_val e1 ltac:(fun v1 => go (CasLCtx v1 v2 :: K) e0)
-     | go (CasMCtx e0 v2 :: K) e1 ])
-  | CAS ?e0 ?e1 ?e2 => go (CasRCtx e0 e1 :: K) e2
-  | FAA ?e1 ?e2 => reshape_val e2 ltac:(fun v2 => go (FaaLCtx v2 :: K) e1)
-  | FAA ?e1 ?e2 => go (FaaRCtx e1 :: K) e2
-  | _ =>
-      lazymatch b with
-      | false => fail
-      | true  => tac K e
-      end
-  end in go (@nil ectx_item) e.
-
-Local Lemma head_step_into_val e σ e' v' σ' efs :
-  IntoVal e' v' →
-  head_step e σ (of_val v') σ' efs →
-  head_step e σ e' σ' efs.
-Proof.
-  intros Hval Hstep. by rewrite Hval in Hstep.
-Qed.
+From iris_time.heap_lang Require Export lang tactics.
 
 Ltac prim_step :=
   lazymatch goal with
-  | |- prim_step ?e _ _ _ _ =>
-      reshape_expr_ordered true e ltac:(fun K e' =>
-        esplit with K e' _ ; [ reflexivity | reflexivity | ] ;
-        (idtac + (eapply head_step_into_val; [apply _|])) ; econstructor
+  | |- prim_step ?e _ _ _ _ _ =>
+      reshape_expr true e ltac:(fun K e' =>
+        esplit with K e' _ ; [ reflexivity | reflexivity | ] ; econstructor
       )
-  end ;
-  simpl_to_of_val.
+  end.
