theories/heap_lang/adequacy.v
@@ -1,0 +1,25 @@
+From iris.program_logic Require Export weakestpre adequacy.
+From iris.algebra Require Import auth.
+From iris_time.heap_lang Require Import proofmode notation.
+From iris.proofmode Require Import tactics.
+Set Default Proof Using "Type".
+
+Class heapPreG Σ := HeapPreG {
+  heap_preG_iris :> invPreG Σ;
+  heap_preG_heap :> gen_heapPreG loc val Σ
+}.
+
+Definition heapΣ : gFunctors := #[invΣ; gen_heapΣ loc val].
+Instance subG_heapPreG {Σ} : subG heapΣ Σ → heapPreG Σ.
+Proof. solve_inG. Qed.
+
+Definition heap_adequacy Σ `{heapPreG Σ} s e σ φ :
+  (∀ `{heapG Σ}, WP e @ s; ⊤ {{ v, ⌜φ v⌝ }}%I) →
+  adequate s e σ (λ v _, φ v).
+Proof.
+  intros Hwp; eapply (wp_adequacy _ _); iIntros (??) "".
+  iMod (gen_heap_init σ) as (?) "Hh".
+  iModIntro.
+  iExists (λ σ κs, (gen_heap_ctx σ)%I). iFrame.
+  iApply (Hwp (HeapG _ _ _)).
+Qed.
