theories/heap_lang/lib/assert.v
@@ -1,0 +1,18 @@
+From iris.program_logic Require Export weakestpre.
+From iris_time.heap_lang Require Export lang.
+From iris.proofmode Require Import tactics.
+From iris_time.heap_lang Require Import proofmode notation.
+Set Default Proof Using "Type".
+
+Definition assert : val :=
+  λ: "v", if: "v" #() then #() else #0 #0. (* #0 #0 is unsafe *)
+(* just below ;; *)
+Notation "'assert:' e" := (assert (λ: <>, e))%E (at level 99) : expr_scope.
+
+Lemma wp_assert `{heapG Σ} E (Φ : val → iProp Σ) e :
+  WP e @ E {{ v, ⌜v = #true⌝ ∧ ▷ Φ #() }} -∗
+  WP assert (LamV BAnon e)%V @ E {{ Φ }}.
+Proof.
+  iIntros "HΦ". wp_lam.
+  wp_apply (wp_wand with "HΦ"). iIntros (v) "[% ?]"; subst. by wp_if.
+Qed.
