theories/heap_lang/lifting.v
@@ -1,0 +1,228 @@
+From iris.algebra Require Import auth gmap.
+From iris.base_logic Require Export gen_heap.
+From iris.program_logic Require Export weakestpre.
+From iris.program_logic Require Import ectx_lifting.
+From iris_time.heap_lang Require Export lang.
+From iris_time.heap_lang Require Import tactics.
+From iris.proofmode Require Import tactics.
+From stdpp Require Import fin_maps.
+Set Default Proof Using "Type".
+
+Class heapG Σ := HeapG {
+  heapG_invG : invG Σ;
+  heapG_gen_heapG :> gen_heapG loc val Σ
+}.
+
+Instance heapG_irisG `{heapG Σ} : irisG heap_lang Σ := {
+  iris_invG := heapG_invG;
+  state_interp σ κs _ := gen_heap_ctx σ;
+  fork_post _ := True%I
+}.
+
+(** Override the notations so that scopes and coercions work out *)
+Notation "l ↦{ q } v" := (mapsto (L:=loc) (V:=val) l q v%V)
+  (at level 20, q at level 50, format "l  ↦{ q }  v") : bi_scope.
+Notation "l ↦ v" :=
+  (mapsto (L:=loc) (V:=val) l 1 v%V) (at level 20) : bi_scope.
+Notation "l ↦{ q } -" := (∃ v, l ↦{q} v)%I
+  (at level 20, q at level 50, format "l  ↦{ q }  -") : bi_scope.
+Notation "l ↦ -" := (l ↦{1} -)%I (at level 20) : bi_scope.
+
+(** The tactic [inv_head_step] performs inversion on hypotheses of the shape
+[head_step]. The tactic will discharge head-reductions starting from values, and
+simplifies hypothesis related to conversions from and to values, and finite map
+operations. This tactic is slightly ad-hoc and tuned for proving our lifting
+lemmas. *)
+Ltac inv_head_step :=
+  repeat match goal with
+  | _ => progress simplify_map_eq/= (* simplify memory stuff *)
+  | H : to_val _ = Some _ |- _ => apply of_to_val in H
+  | H : head_step ?e _ _ _ _ _ |- _ =>
+     try (is_var e; fail 1); (* inversion yields many goals if [e] is a variable
+     and can thus better be avoided. *)
+     inversion H; subst; clear H
+  end.
+
+Local Hint Extern 0 (head_reducible _ _) => eexists _, _, _, _; simpl.
+Local Hint Extern 0 (head_reducible_no_obs _ _) => eexists _, _, _; simpl.
+
+(* [simpl apply] is too stupid, so we need extern hints here. *)
+Local Hint Extern 1 (head_step _ _ _ _ _ _) => econstructor.
+Local Hint Extern 0 (head_step (CAS _ _ _) _ _ _ _ _) => eapply CasSucS.
+Local Hint Extern 0 (head_step (CAS _ _ _) _ _ _ _ _) => eapply CasFailS.
+Local Hint Extern 0 (head_step (Alloc _) _ _ _ _ _) => apply alloc_fresh.
+Local Hint Resolve to_of_val.
+
+Global Instance into_val_val v : IntoVal (Val v) v.
+Proof. done. Qed.
+Global Instance as_val_val v : AsVal (Val v).
+Proof. by eexists. Qed.
+
+Local Ltac solve_atomic :=
+  apply strongly_atomic_atomic, ectx_language_atomic;
+    [inversion 1; naive_solver
+    |apply ectxi_language_sub_redexes_are_values; intros [] **; naive_solver].
+
+Global Instance alloc_atomic s v : Atomic s (Alloc (Val v)).
+Proof. solve_atomic. Qed.
+Global Instance load_atomic s v : Atomic s (Load (Val v)).
+Proof. solve_atomic. Qed.
+Global Instance store_atomic s v1 v2 : Atomic s (Store (Val v1) (Val v2)).
+Proof. solve_atomic. Qed.
+Global Instance cas_atomic s v0 v1 v2 : Atomic s (CAS (Val v0) (Val v1) (Val v2)).
+Proof. solve_atomic. Qed.
+Global Instance faa_atomic s v1 v2 : Atomic s (FAA (Val v1) (Val v2)).
+Proof. solve_atomic. Qed.
+Global Instance fork_atomic s e : Atomic s (Fork e).
+Proof. solve_atomic. Qed.
+Global Instance skip_atomic s  : Atomic s Skip.
+Proof. solve_atomic. Qed.
+
+Local Ltac solve_exec_safe := intros; subst; do 3 eexists; econstructor; eauto.
+Local Ltac solve_exec_puredet := simpl; intros; by inv_head_step.
+Local Ltac solve_pure_exec :=
+  subst; intros ?; apply nsteps_once, pure_head_step_pure_step;
+    constructor; [solve_exec_safe | solve_exec_puredet].
+
+Class AsRecV (v : val) (f x : binder) (erec : expr) :=
+  as_recv : v = RecV f x erec.
+Global Instance AsRecV_recv f x e : AsRecV (RecV f x e) f x e := eq_refl.
+
+(* Pure reductions are automatically performed before any wp_ tactics
+   handling impure operations. Since we do not want these tactics to
+   unfold locked terms, we do not register this instance explicitely,
+   but only activate it by hand in the `wp_rec` tactic, where we
+   *actually* want it to unlock. *)
+Lemma AsRecV_recv_locked v f x e :
+  AsRecV v f x e → AsRecV (locked v) f x e.
+Proof. by unlock. Qed.
+
+Global Instance pure_recc f x (erec : expr) :
+  PureExec True 1 (Rec f x erec) (Val $ RecV f x erec).
+Proof. solve_pure_exec. Qed.
+Global Instance pure_pairc (v1 v2 : val) :
+  PureExec True 1 (Pair (Val v1) (Val v2)) (Val $ PairV v1 v2).
+Proof. solve_pure_exec. Qed.
+Global Instance pure_injlc (v : val) :
+  PureExec True 1 (InjL $ Val v) (Val $ InjLV v).
+Proof. solve_pure_exec. Qed.
+Global Instance pure_injrc (v : val) :
+  PureExec True 1 (InjR $ Val v) (Val $ InjRV v).
+Proof. solve_pure_exec. Qed.
+
+Global Instance pure_beta f x (erec : expr) (v1 v2 : val) `{AsRecV v1 f x erec} :
+  PureExec True 1 (App (Val v1) (Val v2)) (subst' x v2 (subst' f v1 erec)).
+Proof. unfold AsRecV in *. solve_pure_exec. Qed.
+
+Global Instance pure_unop op v v' :
+  PureExec (un_op_eval op v = Some v') 1 (UnOp op (Val v)) (Val v').
+Proof. solve_pure_exec. Qed.
+
+Global Instance pure_binop op v1 v2 v' :
+  PureExec (bin_op_eval op v1 v2 = Some v') 1 (BinOp op (Val v1) (Val v2)) (Val v').
+Proof. solve_pure_exec. Qed.
+
+Global Instance pure_if_true e1 e2 : PureExec True 1 (If (Val $ LitV $ LitBool true) e1 e2) e1.
+Proof. solve_pure_exec. Qed.
+
+Global Instance pure_if_false e1 e2 : PureExec True 1 (If (Val $ LitV  $ LitBool false) e1 e2) e2.
+Proof. solve_pure_exec. Qed.
+
+Global Instance pure_fst v1 v2 :
+  PureExec True 1 (Fst (Val $ PairV v1 v2)) (Val v1).
+Proof. solve_pure_exec. Qed.
+
+Global Instance pure_snd v1 v2 :
+  PureExec True 1 (Snd (Val $ PairV v1 v2)) (Val v2).
+Proof. solve_pure_exec. Qed.
+
+Global Instance pure_case_inl v e1 e2 :
+  PureExec True 1 (Case (Val $ InjLV v) e1 e2) (App e1 (Val v)).
+Proof. solve_pure_exec. Qed.
+
+Global Instance pure_case_inr v e1 e2 :
+  PureExec True 1 (Case (Val $ InjRV v) e1 e2) (App e2 (Val v)).
+Proof. solve_pure_exec. Qed.
+
+Section lifting.
+Context `{heapG Σ}.
+Implicit Types P Q : iProp Σ.
+Implicit Types Φ : val → iProp Σ.
+Implicit Types efs : list expr.
+Implicit Types σ : state.
+
+(** Fork: Not using Texan triples to avoid some unnecessary [True] *)
+Lemma wp_fork s E e Φ :
+  ▷ WP e @ s; ⊤ {{ _, True }} -∗ ▷ Φ (LitV LitUnit) -∗ WP Fork e @ s; E {{ Φ }}.
+Proof.
+  iIntros "He HΦ". iApply wp_lift_atomic_head_step; [done|].
+  iIntros (σ1 κ κs n) "Hσ !>"; iSplit; first by eauto.
+  iNext; iIntros (v2 σ2 efs Hstep); inv_head_step. by iFrame.
+Qed.
+
+(** Heap *)
+Lemma wp_alloc s E v :
+  {{{ True }}} Alloc (Val v) @ s; E {{{ l, RET LitV (LitLoc l); l ↦ v }}}.
+Proof.
+  iIntros (Φ) "_ HΦ". iApply wp_lift_atomic_head_step_no_fork; auto.
+  iIntros (σ1 κ κs n) "Hσ !>"; iSplit; first by auto.
+  iNext; iIntros (v2 σ2 efs Hstep); inv_head_step.
+  iMod (@gen_heap_alloc with "Hσ") as "[Hσ Hl]"; first done.
+  iModIntro; iSplit=> //. iFrame. by iApply "HΦ".
+Qed.
+
+Lemma wp_load s E l q v :
+  {{{ ▷ l ↦{q} v }}} Load (Val $ LitV $ LitLoc l) @ s; E {{{ RET v; l ↦{q} v }}}.
+Proof.
+  iIntros (Φ) ">Hl HΦ". iApply wp_lift_atomic_head_step_no_fork; auto.
+  iIntros (σ1 κ κs n) "Hσ !>". iDestruct (@gen_heap_valid with "Hσ Hl") as %?.
+  iSplit; first by eauto. iNext; iIntros (v2 σ2 efs Hstep); inv_head_step.
+  iModIntro; iSplit=> //. iFrame. by iApply "HΦ".
+Qed.
+
+Lemma wp_store s E l v' v :
+  {{{ ▷ l ↦ v' }}} Store (Val $ LitV (LitLoc l)) (Val v) @ s; E
+  {{{ RET LitV LitUnit; l ↦ v }}}.
+Proof.
+  iIntros (Φ) ">Hl HΦ".
+  iApply wp_lift_atomic_head_step_no_fork; auto.
+  iIntros (σ1 κ κs n) "Hσ !>". iDestruct (@gen_heap_valid with "Hσ Hl") as %?.
+  iSplit; first by eauto. iNext; iIntros (v2 σ2 efs Hstep); inv_head_step.
+  iMod (@gen_heap_update with "Hσ Hl") as "[$ Hl]".
+  iModIntro. iSplit=>//. iFrame. by iApply "HΦ".
+Qed.
+
+Lemma wp_cas_fail s E l q v' v1 v2 :
+  v' ≠ v1 → vals_cas_compare_safe v' v1 →
+  {{{ ▷ l ↦{q} v' }}} CAS (Val $ LitV $ LitLoc l) (Val v1) (Val v2) @ s; E
+  {{{ RET LitV (LitBool false); l ↦{q} v' }}}.
+Proof.
+  iIntros (?? Φ) ">Hl HΦ". iApply wp_lift_atomic_head_step_no_fork; auto.
+  iIntros (σ1 κ κs n) "Hσ !>". iDestruct (@gen_heap_valid with "Hσ Hl") as %?.
+  iSplit; first by eauto. iNext; iIntros (v2' σ2 efs Hstep); inv_head_step.
+  iModIntro; iSplit=> //. iFrame. by iApply "HΦ".
+Qed.
+
+Lemma wp_cas_suc s E l v1 v2 :
+  vals_cas_compare_safe v1 v1 →
+  {{{ ▷ l ↦ v1 }}} CAS (Val $ LitV $ LitLoc l) (Val v1) (Val v2) @ s; E
+  {{{ RET LitV (LitBool true); l ↦ v2 }}}.
+Proof.
+  iIntros (? Φ) ">Hl HΦ". iApply wp_lift_atomic_head_step_no_fork; auto.
+  iIntros (σ1 κ κs n) "Hσ !>". iDestruct (@gen_heap_valid with "Hσ Hl") as %?.
+  iSplit; first by eauto. iNext; iIntros (v2' σ2 efs Hstep); inv_head_step.
+  iMod (@gen_heap_update with "Hσ Hl") as "[$ Hl]".
+  iModIntro. iSplit=>//. iFrame. by iApply "HΦ".
+Qed.
+
+Lemma wp_faa s E l i1 i2 :
+  {{{ ▷ l ↦ LitV (LitInt i1) }}} FAA (Val $ LitV $ LitLoc l) (Val $ LitV $ LitInt i2) @ s; E
+  {{{ RET LitV (LitInt i1); l ↦ LitV (LitInt (i1 + i2)) }}}.
+Proof.
+  iIntros (Φ) ">Hl HΦ". iApply wp_lift_atomic_head_step_no_fork; auto.
+  iIntros (σ1 κ κs n) "Hσ !>". iDestruct (@gen_heap_valid with "Hσ Hl") as %?.
+  iSplit; first by eauto. iNext; iIntros (v2' σ2 efs Hstep); inv_head_step.
+  iMod (@gen_heap_update with "Hσ Hl") as "[$ Hl]".
+  iModIntro. iSplit=>//. iFrame. by iApply "HΦ".
+Qed.
+End lifting.
