theories/heap_lang/proofmode.v
@@ -1,0 +1,365 @@
+From iris.program_logic Require Export weakestpre.
+From iris.proofmode Require Import coq_tactics reduction.
+From iris.proofmode Require Export tactics.
+From iris_time.heap_lang Require Export tactics lifting.
+From iris_time.heap_lang Require Import notation.
+Set Default Proof Using "Type".
+Import uPred.
+
+Lemma tac_wp_expr_eval `{heapG Σ} Δ s E Φ e e' :
+  (∀ (e'':=e'), e = e'') →
+  envs_entails Δ (WP e' @ s; E {{ Φ }}) → envs_entails Δ (WP e @ s; E {{ Φ }}).
+Proof. by intros ->. Qed.
+
+Tactic Notation "wp_expr_eval" tactic(t) :=
+  iStartProof;
+  lazymatch goal with
+  | |- envs_entails _ (wp ?s ?E ?e ?Q) =>
+    eapply tac_wp_expr_eval;
+      [let x := fresh in intros x; t; unfold x; reflexivity|]
+  | _ => fail "wp_expr_eval: not a 'wp'"
+  end.
+
+Ltac wp_expr_simpl := wp_expr_eval simpl.
+
+Lemma tac_wp_pure `{heapG Σ} Δ Δ' s E e1 e2 φ n Φ :
+  PureExec φ n e1 e2 →
+  φ →
+  MaybeIntoLaterNEnvs n Δ Δ' →
+  envs_entails Δ' (WP e2 @ s; E {{ Φ }}) →
+  envs_entails Δ (WP e1 @ s; E {{ Φ }}).
+Proof.
+  rewrite envs_entails_eq=> ??? HΔ'. rewrite into_laterN_env_sound /=.
+  rewrite HΔ' -lifting.wp_pure_step_later //.
+Qed.
+
+Lemma tac_wp_value `{heapG Σ} Δ s E Φ v :
+  envs_entails Δ (Φ v) → envs_entails Δ (WP (Val v) @ s; E {{ Φ }}).
+Proof. rewrite envs_entails_eq=> ->. by apply wp_value. Qed.
+
+Ltac wp_value_head :=
+  eapply tac_wp_value; reduction.pm_prettify.
+
+Tactic Notation "wp_pure" open_constr(efoc) :=
+  iStartProof;
+  lazymatch goal with
+  | |- envs_entails _ (wp ?s ?E ?e ?Q) =>
+    let e := eval simpl in e in
+    reshape_expr false e ltac:(fun K e' =>
+      unify e' efoc;
+      eapply (tac_wp_pure _ _ _ _ (fill K e'));
+      [iSolveTC                       (* PureExec *)
+      |try fast_done                  (* The pure condition for PureExec *)
+      |iSolveTC                       (* IntoLaters *)
+      |wp_expr_simpl; try wp_value_head (* new goal *)
+      ])
+    || fail "wp_pure: cannot find" efoc "in" e "or" efoc "is not a redex"
+  | _ => fail "wp_pure: not a 'wp'"
+  end.
+
+(* TODO: do this in one go, without [repeat]. *)
+Ltac wp_pures :=
+  iStartProof;
+  repeat (wp_pure _; []). (* The `;[]` makes sure that no side-condition
+                             magically spawns. *)
+
+(* The handling of beta-reductions with wp_rec needs special care in
+  order to allow it to unlock locked `RecV` values: We first put
+  `AsRecV_recv_locked` in the current environment so that it can be
+  used as an instance by the typeclass resolution system, then we
+  perform the reduction, and finally we clear this new hypothesis.
+
+  The reason is that we do not want impure wp_ tactics to unfold
+  locked terms, while we want them to execute arbitrary pure steps. *)
+Tactic Notation "wp_rec" :=
+  let H := fresh in
+  assert (H := AsRecV_recv_locked);
+  wp_pure (App _ _);
+  clear H.
+
+Tactic Notation "wp_if" := wp_pure (If _ _ _).
+Tactic Notation "wp_if_true" := wp_pure (If (LitV (LitBool true)) _ _).
+Tactic Notation "wp_if_false" := wp_pure (If (LitV (LitBool false)) _ _).
+Tactic Notation "wp_unop" := wp_pure (UnOp _ _).
+Tactic Notation "wp_binop" := wp_pure (BinOp _ _ _).
+Tactic Notation "wp_op" := wp_unop || wp_binop.
+Tactic Notation "wp_lam" := wp_rec.
+Tactic Notation "wp_let" := wp_pure (Rec BAnon (BNamed _) _); wp_lam.
+Tactic Notation "wp_seq" := wp_pure (Rec BAnon BAnon _); wp_lam.
+Tactic Notation "wp_proj" := wp_pure (Fst _) || wp_pure (Snd _).
+Tactic Notation "wp_case" := wp_pure (Case _ _ _).
+Tactic Notation "wp_match" := wp_case; wp_pure (Rec _ _ _); wp_lam.
+Tactic Notation "wp_inj" := wp_pure (InjL _) || wp_pure (InjR _).
+Tactic Notation "wp_pair" := wp_pure (Pair _ _).
+Tactic Notation "wp_closure" := wp_pure (Rec _ _ _).
+
+Lemma tac_wp_bind `{heapG Σ} K Δ s E Φ e f :
+  f = (λ e, fill K e) → (* as an eta expanded hypothesis so that we can `simpl` it *)
+  envs_entails Δ (WP e @ s; E {{ v, WP f (Val v) @ s; E {{ Φ }} }})%I →
+  envs_entails Δ (WP fill K e @ s; E {{ Φ }}).
+Proof. rewrite envs_entails_eq=> -> ->. by apply: wp_bind. Qed.
+
+Ltac wp_bind_core K :=
+  lazymatch eval hnf in K with
+  | [] => idtac
+  | _ => eapply (tac_wp_bind K); [simpl; reflexivity|reduction.pm_prettify]
+  end.
+
+Tactic Notation "wp_bind" open_constr(efoc) :=
+  iStartProof;
+  lazymatch goal with
+  | |- envs_entails _ (wp ?s ?E ?e ?Q) =>
+    reshape_expr false e ltac:(fun K e' => unify e' efoc; wp_bind_core K)
+    || fail "wp_bind: cannot find" efoc "in" e
+  | _ => fail "wp_bind: not a 'wp'"
+  end.
+
+(** Heap tactics *)
+Section heap.
+Context `{WordSize, heapG Σ}.
+Implicit Types P Q : iProp Σ.
+Implicit Types Φ : val → iProp Σ.
+Implicit Types Δ : envs (uPredI (iResUR Σ)).
+Implicit Types v : val.
+Implicit Types z : Z.
+
+Lemma tac_wp_alloc Δ Δ' s E j K v Φ :
+  MaybeIntoLaterNEnvs 1 Δ Δ' →
+  (∀ l, ∃ Δ'',
+    envs_app false (Esnoc Enil j (l ↦ v)) Δ' = Some Δ'' ∧
+    envs_entails Δ'' (WP fill K (Val $ LitV l) @ s; E {{ Φ }})) →
+  envs_entails Δ (WP fill K (Alloc v) @ s; E {{ Φ }}).
+Proof.
+  rewrite envs_entails_eq=> ? HΔ.
+  rewrite -wp_bind. eapply wand_apply; first exact: wp_alloc.
+  rewrite left_id into_laterN_env_sound; apply later_mono, forall_intro=> l.
+  destruct (HΔ l) as (Δ''&?&HΔ'). rewrite envs_app_sound //; simpl.
+  by rewrite right_id HΔ'.
+Qed.
+
+Lemma tac_wp_load Δ Δ' s E i K l q v Φ :
+  MaybeIntoLaterNEnvs 1 Δ Δ' →
+  envs_lookup i Δ' = Some (false, l ↦{q} v)%I →
+  envs_entails Δ' (WP fill K (Val v) @ s; E {{ Φ }}) →
+  envs_entails Δ (WP fill K (Load (LitV l)) @ s; E {{ Φ }}).
+Proof.
+  rewrite envs_entails_eq=> ???.
+  rewrite -wp_bind. eapply wand_apply; first exact: wp_load.
+  rewrite into_laterN_env_sound -later_sep envs_lookup_split //; simpl.
+  by apply later_mono, sep_mono_r, wand_mono.
+Qed.
+
+Lemma tac_wp_store Δ Δ' Δ'' s E i K l v v' Φ :
+  MaybeIntoLaterNEnvs 1 Δ Δ' →
+  envs_lookup i Δ' = Some (false, l ↦ v)%I →
+  envs_simple_replace i false (Esnoc Enil i (l ↦ v')) Δ' = Some Δ'' →
+  envs_entails Δ'' (WP fill K (Val $ LitV LitUnit) @ s; E {{ Φ }}) →
+  envs_entails Δ (WP fill K (Store (LitV l) (Val v')) @ s; E {{ Φ }}).
+Proof.
+  rewrite envs_entails_eq=> ????.
+  rewrite -wp_bind. eapply wand_apply; first by eapply wp_store.
+  rewrite into_laterN_env_sound -later_sep envs_simple_replace_sound //; simpl.
+  rewrite right_id. by apply later_mono, sep_mono_r, wand_mono.
+Qed.
+
+Lemma tac_wp_cas Δ Δ' Δ'' s E i K l v v1 v2 Φ :
+  MaybeIntoLaterNEnvs 1 Δ Δ' →
+  envs_lookup i Δ' = Some (false, l ↦ v)%I →
+  envs_simple_replace i false (Esnoc Enil i (l ↦ v2)) Δ' = Some Δ'' →
+  vals_cas_compare_safe v v1 →
+  (v = v1 → envs_entails Δ'' (WP fill K (Val $ LitV true) @ s; E {{ Φ }})) →
+  (v ≠ v1 → envs_entails Δ' (WP fill K (Val $ LitV false) @ s; E {{ Φ }})) →
+  envs_entails Δ (WP fill K (CAS (LitV l) (Val v1) (Val v2)) @ s; E {{ Φ }}).
+Proof.
+  rewrite envs_entails_eq=> ???? Hsuc Hfail. destruct (decide (v = v1)) as [<-|Hne].
+  - rewrite -wp_bind. eapply wand_apply; first exact: wp_cas_suc.
+    rewrite into_laterN_env_sound -later_sep /= {1}envs_simple_replace_sound //; simpl.
+    apply later_mono, sep_mono_r. rewrite right_id. apply wand_mono; auto.
+  - rewrite -wp_bind. eapply wand_apply.
+    { eapply wp_cas_fail; eauto. }
+    rewrite into_laterN_env_sound -later_sep /= {1}envs_lookup_split //; simpl.
+    apply later_mono, sep_mono_r. apply wand_mono; auto.
+Qed.
+
+Lemma tac_wp_cas_fail Δ Δ' s E i K l q v v1 v2 Φ :
+  MaybeIntoLaterNEnvs 1 Δ Δ' →
+  envs_lookup i Δ' = Some (false, l ↦{q} v)%I →
+  v ≠ v1 → vals_cas_compare_safe v v1 →
+  envs_entails Δ' (WP fill K (Val $ LitV false) @ s; E {{ Φ }}) →
+  envs_entails Δ (WP fill K (CAS (LitV l) v1 v2) @ s; E {{ Φ }}).
+Proof.
+  rewrite envs_entails_eq=> ?????.
+  rewrite -wp_bind. eapply wand_apply; first exact: wp_cas_fail.
+  rewrite into_laterN_env_sound -later_sep envs_lookup_split //; simpl.
+  by apply later_mono, sep_mono_r, wand_mono.
+Qed.
+
+Lemma tac_wp_cas_suc Δ Δ' Δ'' s E i K l v v1 v2 Φ :
+  MaybeIntoLaterNEnvs 1 Δ Δ' →
+  envs_lookup i Δ' = Some (false, l ↦ v)%I →
+  envs_simple_replace i false (Esnoc Enil i (l ↦ v2)) Δ' = Some Δ'' →
+  v = v1 → val_is_unboxed v →
+  envs_entails Δ'' (WP fill K (Val $ LitV true) @ s; E {{ Φ }}) →
+  envs_entails Δ (WP fill K (CAS (LitV l) v1 v2) @ s; E {{ Φ }}).
+Proof.
+  rewrite envs_entails_eq=> ??????; subst.
+  rewrite -wp_bind. eapply wand_apply.
+  { eapply wp_cas_suc; eauto. by left. }
+  rewrite into_laterN_env_sound -later_sep envs_simple_replace_sound //; simpl.
+  rewrite right_id. by apply later_mono, sep_mono_r, wand_mono.
+Qed.
+
+Lemma tac_wp_faa Δ Δ' Δ'' s E i K l z1 z2 Φ :
+  MaybeIntoLaterNEnvs 1 Δ Δ' →
+  envs_lookup i Δ' = Some (false, l ↦ LitV z1)%I →
+  envs_simple_replace i false (Esnoc Enil i (l ↦ LitV (z1 + z2))) Δ' = Some Δ'' →
+  envs_entails Δ'' (WP fill K (Val $ LitV z1) @ s; E {{ Φ }}) →
+  envs_entails Δ (WP fill K (FAA (LitV l) (LitV z2)) @ s; E {{ Φ }}).
+Proof.
+  rewrite envs_entails_eq=> ????.
+  rewrite -wp_bind. eapply wand_apply; first exact: (wp_faa _ _ _ z1 z2).
+  rewrite into_laterN_env_sound -later_sep envs_simple_replace_sound //; simpl.
+  rewrite right_id. by apply later_mono, sep_mono_r, wand_mono.
+Qed.
+End heap.
+
+Tactic Notation "wp_apply" open_constr(lem) :=
+  wp_pures;
+  iPoseProofCore lem as false true (fun H =>
+    lazymatch goal with
+    | |- envs_entails _ (wp ?s ?E ?e ?Q) =>
+      reshape_expr false e ltac:(fun K e' =>
+        wp_bind_core K; iApplyHyp H; try iNext; try wp_expr_simpl) ||
+      lazymatch iTypeOf H with
+      | Some (_,?P) => fail "wp_apply: cannot apply" P
+      end
+    | _ => fail "wp_apply: not a 'wp'"
+    end).
+
+Tactic Notation "wp_alloc" ident(l) "as" constr(H) :=
+  let Htmp := iFresh in
+  let finish _ :=
+    first [intros l | fail 1 "wp_alloc:" l "not fresh"];
+      eexists; split;
+        [pm_reflexivity || fail "wp_alloc:" H "not fresh"
+        |iDestructHyp Htmp as H; wp_expr_simpl; try wp_value_head] in
+  wp_pures;
+  lazymatch goal with
+  | |- envs_entails _ (wp ?s ?E ?e ?Q) =>
+    first
+      [reshape_expr false e ltac:(fun K e' => eapply (tac_wp_alloc _ _ _ _ Htmp K))
+      |fail 1 "wp_alloc: cannot find 'Alloc' in" e];
+    [iSolveTC
+    |finish ()]
+  | _ => fail "wp_alloc: not a 'wp'"
+  end.
+
+Tactic Notation "wp_alloc" ident(l) :=
+  wp_alloc l as "?".
+
+Tactic Notation "wp_load" :=
+  let solve_mapsto _ :=
+    let l := match goal with |- _ = Some (_, (?l ↦{_} _)%I) => l end in
+    iAssumptionCore || fail "wp_load: cannot find" l "↦ ?" in
+  wp_pures;
+  lazymatch goal with
+  | |- envs_entails _ (wp ?s ?E ?e ?Q) =>
+    first
+      [reshape_expr false e ltac:(fun K e' => eapply (tac_wp_load _ _ _ _ _ K))
+      |fail 1 "wp_load: cannot find 'Load' in" e];
+    [iSolveTC
+    |solve_mapsto ()
+    |wp_expr_simpl; try wp_value_head]
+  | _ => fail "wp_load: not a 'wp'"
+  end.
+
+Tactic Notation "wp_store" :=
+  let solve_mapsto _ :=
+    let l := match goal with |- _ = Some (_, (?l ↦{_} _)%I) => l end in
+    iAssumptionCore || fail "wp_store: cannot find" l "↦ ?" in
+  let finish _ := wp_expr_simpl; try wp_value_head in
+  wp_pures;
+  lazymatch goal with
+  | |- envs_entails _ (wp ?s ?E ?e ?Q) =>
+    first
+      [reshape_expr false e ltac:(fun K e' => eapply (tac_wp_store _ _ _ _ _ _ K))
+      |fail 1 "wp_store: cannot find 'Store' in" e];
+    [iSolveTC
+    |solve_mapsto ()
+    |pm_reflexivity
+    |finish ()]
+  | _ => fail "wp_store: not a 'wp'"
+  end.
+
+Tactic Notation "wp_cas" "as" simple_intropattern(H1) "|" simple_intropattern(H2) :=
+  let solve_mapsto _ :=
+    let l := match goal with |- _ = Some (_, (?l ↦{_} _)%I) => l end in
+    iAssumptionCore || fail "wp_cas: cannot find" l "↦ ?" in
+  wp_pures;
+  lazymatch goal with
+  | |- envs_entails _ (wp ?s ?E ?e ?Q) =>
+    first
+      [reshape_expr false e ltac:(fun K e' => eapply (tac_wp_cas _ _ _ _ _ _ K))
+      |fail 1 "wp_cas: cannot find 'CAS' in" e];
+    [iSolveTC
+    |solve_mapsto ()
+    |pm_reflexivity
+    |try (fast_done || (left; fast_done) || (right; fast_done)) (* vals_cas_compare_safe *)
+    |intros H1; wp_expr_simpl; try wp_value_head
+    |intros H2; wp_expr_simpl; try wp_value_head]
+  | _ => fail "wp_cas: not a 'wp'"
+  end.
+
+Tactic Notation "wp_cas_fail" :=
+  let solve_mapsto _ :=
+    let l := match goal with |- _ = Some (_, (?l ↦{_} _)%I) => l end in
+    iAssumptionCore || fail "wp_cas_fail: cannot find" l "↦ ?" in
+  wp_pures;
+  lazymatch goal with
+  | |- envs_entails _ (wp ?s ?E ?e ?Q) =>
+    first
+      [reshape_expr false e ltac:(fun K e' => eapply (tac_wp_cas_fail _ _ _ _ _ K))
+      |fail 1 "wp_cas_fail: cannot find 'CAS' in" e];
+    [iSolveTC
+    |solve_mapsto ()
+    |try congruence
+    |try (fast_done || (left; fast_done) || (right; fast_done)) (* vals_cas_compare_safe *)
+    |simpl; try wp_value_head]
+  | _ => fail "wp_cas_fail: not a 'wp'"
+  end.
+
+Tactic Notation "wp_cas_suc" :=
+  let solve_mapsto _ :=
+    let l := match goal with |- _ = Some (_, (?l ↦{_} _)%I) => l end in
+    iAssumptionCore || fail "wp_cas_suc: cannot find" l "↦ ?" in
+  wp_pures;
+  lazymatch goal with
+  | |- envs_entails _ (wp ?s ?E ?e ?Q) =>
+    first
+      [reshape_expr false e ltac:(fun K e' => eapply (tac_wp_cas_suc _ _ _ _ _ _ K))
+      |fail 1 "wp_cas_suc: cannot find 'CAS' in" e];
+    [iSolveTC
+    |solve_mapsto ()
+    |pm_reflexivity
+    |try congruence
+    |try fast_done (* vals_cas_compare_safe *)
+    |simpl; try wp_value_head]
+  | _ => fail "wp_cas_suc: not a 'wp'"
+  end.
+
+Tactic Notation "wp_faa" :=
+  let solve_mapsto _ :=
+    let l := match goal with |- _ = Some (_, (?l ↦{_} _)%I) => l end in
+    iAssumptionCore || fail "wp_cas_suc: cannot find" l "↦ ?" in
+  wp_pures;
+  lazymatch goal with
+  | |- envs_entails _ (wp ?s ?E ?e ?Q) =>
+    first
+      [reshape_expr false e ltac:(fun K e' => eapply (tac_wp_faa _ _ _ _ _ _ K))
+      |fail 1 "wp_faa: cannot find 'CAS' in" e];
+    [iSolveTC
+    |solve_mapsto ()
+    |pm_reflexivity
+    |wp_expr_simpl; try wp_value_head]
+  | _ => fail "wp_faa: not a 'wp'"
+  end.
