theories/heap_lang/tactics.v
@@ -1,0 +1,49 @@
+From iris_time.heap_lang Require Export lang.
+Set Default Proof Using "Type".
+Import heap_lang.
+
+(** The tactic [reshape_expr e tac] decomposes the expression [e] into an
+evaluation context [K] and a subexpression [e']. It calls the tactic [tac K e']
+for each possible decomposition until [tac] succeeds.
+
+The order parameter specifies the order in which these decompositions are tried.
+If true, contexts are tried starting from the most nested, when false, the
+first tried context is the least nested.
+
+ *)
+Ltac reshape_expr order e tac :=
+  let rec go K e :=
+  match e with
+  | _ =>
+      lazymatch order with
+      | false => tac K e
+      | true  => fail
+      end
+  | App ?e (Val ?v) => go (AppLCtx v :: K) e
+  | App ?e1 ?e2 => go (AppRCtx e1 :: K) e2
+  | UnOp ?op ?e => go (UnOpCtx op :: K) e
+  | BinOp ?op ?e (Val ?v) => go (BinOpLCtx op v :: K) e
+  | BinOp ?op ?e1 ?e2 => go (BinOpRCtx op e1 :: K) e2
+  | If ?e0 ?e1 ?e2 => go (IfCtx e1 e2 :: K) e0
+  | Pair ?e (Val ?v) => go (PairLCtx v :: K) e
+  | Pair ?e1 ?e2 => go (PairRCtx e1 :: K) e2
+  | Fst ?e => go (FstCtx :: K) e
+  | Snd ?e => go (SndCtx :: K) e
+  | InjL ?e => go (InjLCtx :: K) e
+  | InjR ?e => go (InjRCtx :: K) e
+  | Case ?e0 ?e1 ?e2 => go (CaseCtx e1 e2 :: K) e0
+  | Alloc ?e => go (AllocCtx :: K) e
+  | Load ?e => go (LoadCtx :: K) e
+  | Store ?e (Val ?v) => go (StoreLCtx v :: K) e
+  | Store ?e1 ?e2 => go (StoreRCtx e1 :: K) e2
+  | CAS ?e0 (Val ?v1) (Val ?v2) => go (CasLCtx v1 v2 :: K) e0
+  | CAS ?e0 ?e1 (Val ?v2) => go (CasMCtx e0 v2 :: K) e1
+  | CAS ?e0 ?e1 ?e2 => go (CasRCtx e0 e1 :: K) e2
+  | FAA ?e (Val ?v) => go (FaaLCtx v :: K) e
+  | FAA ?e1 ?e2 => go (FaaRCtx e1 :: K) e2
+  | _ =>
+      lazymatch order with
+      | false => fail
+      | true  => tac K e
+      end
+  end in go (@nil ectx_item) e.
